

Linear Equation  $\Rightarrow \hat{y} = mx + b$

points  $\Rightarrow (1, 3)$  and  $(3, 6)$

Initial values  $\Rightarrow m_0 = -1, b_0 = 1$   
 $m_0 = -1$

Learning rate  $\Rightarrow \alpha = 0.1$

Number of data points  $\Rightarrow n = 2$

Cost function (MSE) using the common convention with factor  $\frac{1}{2n}$ :

$$J(m, b) = \frac{1}{2n} \sum_{i=1}^n (y_i - (mx + b))^2$$

for  $n = 2$ , the prefactor is  $\frac{1}{2n}$

$$\Rightarrow \frac{1}{2(2)} = \frac{1}{4} = 0.25$$

Derive gradients

$$\text{From } J(m, b) = \frac{1}{2n} \sum_{i=1}^n (y_i - (mx + b))^2$$

let  $e_i = y_i - (mx + b)$

$$J(m, b) = \frac{1}{2n} \sum_{i=1}^n e_i^2$$

Partial derivative of  $m$ :

$$\frac{\partial J}{\partial m} = \frac{1}{2n} \sum_{i=1}^n 2e_i \cdot \frac{\partial e_i}{\partial m} \quad (\text{chain rule})$$

$$\text{where } e_i = y_i - (mx + b)$$

$$\frac{\partial e_i}{\partial m} = -x$$

$$\text{so } \frac{\partial J}{\partial m} = \frac{1}{2n} \sum_{i=1}^n 2e_i(-x)$$

$$= \frac{1}{n} \sum_{i=1}^n -e_i x$$

Partial derivative of  $b$ :

$$\frac{\partial J}{\partial b} = \frac{1}{2n} \sum_{i=1}^n 2e_i \frac{\partial e_i}{\partial b}$$

$$\text{where } \frac{\partial e_i}{\partial b} = -1$$

$$\text{therefore } \frac{\partial J}{\partial b} = \frac{1}{n} \sum_{i=1}^n -e_i$$

Gradient formulas:

$$\frac{\partial J}{\partial m} = \frac{1}{n} \sum_{i=1}^n x (y_i - (mx + b))$$

$$\frac{\partial J}{\partial b} = \frac{1}{n} \sum_{i=1}^n (y_i - (mx + b))$$

Update rules (gradient descent):

$$m_{\text{new}} = m_{\text{old}} - \alpha \frac{\partial J}{\partial m}$$

$$b_{\text{new}} = b_{\text{old}} - \alpha \frac{\partial J}{\partial b}$$

Iteration

Given information:

$$m_0 = -1, b_0 = 1, \text{ points } (1, 3), (3, 6)$$

Let's compute initial predictions:

$$\text{for } x_1 = 1, \hat{y}_1 = m_0 x_1 + b_0$$

$$= (-1)(1) + 1$$

$$= 0$$



For  $x_2 = 3$ ,  $\hat{y}_2 = m_0 x_2 + b_0$   
 $= (-1)(3) + 1$   
 $= -2$

Error<sub>1</sub> =  $y_1 - \hat{y}_1 = 3 - 0 = 3$

Error<sub>2</sub> =  $y_2 - \hat{y}_2 = 6 - (-2) = 8$

Compute cost:

$$J_0 = \frac{1}{2n} \sum_{i=1}^n (y_i - \hat{y}_i)^2$$

$$J_0 = \frac{1}{2(2)} ((\text{error}_1 + \text{error}_2)^2)$$

$$= \frac{1}{4} (3^2 + 8^2)$$

$$= \frac{73}{4} = 18.25$$

Let's compute gradient:

$$\frac{\partial J}{\partial m} = \frac{1}{n} \sum_{i=1}^n e_i x_i, n=2$$

and

$$\frac{\partial J}{\partial b} = \frac{1}{n} \sum_{i=1}^n e_i$$

For  $\frac{\partial J}{\partial m} = \frac{1}{n} \sum_{i=1}^n e_i x_i$   
 $= \frac{1}{n} (\text{error}_1 x_1 + \text{error}_2 x_2)$   
 $= \frac{1}{2} (3(1) + 8(3))$   
 $= \frac{1}{2} (3 + 24)$   
 $= \frac{27}{2} = 13.5$

For  $\frac{\partial J}{\partial b} = \frac{1}{n} \sum_{i=1}^n e_i$   
 $= \frac{1}{n} (\text{error}_1 + \text{error}_2)$   
 $= \frac{1}{2} (3 + 8)$   
 $= \frac{11}{2} = 5.5$

Next, updating the parameters:

$$m_1 = m_0 - \alpha \cdot \frac{\partial J}{\partial m}$$

$$= -1 - (0.1)(-13.5)$$

$$= 0.35$$

$$b_1 = b_0 - \alpha \cdot \frac{\partial J}{\partial b}$$

$$= 1 - (0.1)(-5.5)$$

$$= 1.55$$

After the iteration, this is our new values:

$$m_{\text{new}} = 0.35$$

$$b_{\text{new}} = 1.55$$



Given  $m_0 = -1$  and  $b_0 = 1$  and also  $m_{\text{new}} = 0.35$  and  $b_{\text{new}} = 1.55$  by calculation our new values of  $m$  and  $b$  are increasing where by  $m$  we are increasing by the change of  $+1.35$  and  $b$  is increasing by the change of  $+0.55$ . So,

Thus, the values of  $m$  and  $b$  are moving towards reducing the error because of the negative gradient  $(-13.5, -5.5)$  combined with the gradient descent are the one pushing or moves the parameters in the correct direction to fit the line of the points  $(1, 3)$  and  $(3, 6)$ .